Almost there with the bloom filter proof

bloom-filter/BloomFilter.fst
@@ -25,13 +25,13 @@ let _KEY_MASK: (v:u32{U32.v v = 0xfff}) =
   assert_norm (value = 0xffful);
   value
 
-noeq type bloom_storage_u8 = {
+type bloom_storage_u8 = {
   counters: array u8 _ARRAY_SIZE;
   ghost_state: spec_bloom_storage_u8
 }
 
 
-let valid_index (bf: bloom_storage_u8) = i:usize{Usize.(i <^ array_length bf.counters)}
+let valid_index = i:usize{Usize.(i <^ _ARRAY_SIZE)}
 
 val hash1: u32 -> r:u32{U32.(r <^ _ARRAY_SIZE)}
 let hash1 hash =
@@ -51,7 +51,7 @@ let first_slot_index (hash: u32) : r:usize{Usize.(r <^ _ARRAY_SIZE)} =
 let second_slot_index (hash: u32) : usize =
   hash2 hash
 
-val slot_is_empty: bf:bloom_storage_u8 -> valid_index bf -> Tot bool
+val slot_is_empty: bf:bloom_storage_u8 -> valid_index -> Tot bool
 let slot_is_empty bf idx =
   (array_index bf.counters idx) = 0uy
 
@@ -61,22 +61,35 @@ let first_slot_is_empty bf hash = slot_is_empty bf (first_slot_index hash)
 val second_slot_is_empty : bf:bloom_storage_u8 -> u32 -> Tot bool
 let second_slot_is_empty bf hash = slot_is_empty bf (second_slot_index hash)
 
+val might_contain_hash: bf:bloom_storage_u8 -> u32 -> bool
+let might_contain_hash bf hash =
+  not (first_slot_is_empty bf hash) &&
+  not (second_slot_is_empty bf hash)
+
+let modified_only_one_slot
+  (old_bf:bloom_storage_u8)
+  (new_bf:bloom_storage_u8)
+  (idx:valid_index) =
+  forall (idx':valid_index{idx <> idx'}).
+  array_index new_bf.counters idx' = array_index old_bf.counters idx'
+
 val adjust_slot:
   bf:bloom_storage_u8 ->
-  idx:valid_index bf ->
+  idx:valid_index ->
   increment:bool{if not increment then not (slot_is_empty bf idx) else true } ->
   Tot (new_bf:bloom_storage_u8{
-    forall (idx':valid_index bf{idx <> idx'}). (
-      array_index new_bf.counters idx' = array_index bf.counters idx'
-    )
+    modified_only_one_slot bf new_bf idx /\
+    begin if increment then
+      not (slot_is_empty new_bf idx)
+    else
+      true
+    end
   })
 let adjust_slot bf idx increment =
   let slot = array_index bf.counters idx in
   if slot <> 0xffuy then
     if increment then begin
-      let new_counters = array_update bf.counters idx U8.(slot +^ 1uy)  in
-      lemma_array_update u8 _ARRAY_SIZE bf.counters idx U8.(slot +^ 1uy);
-      { bf with counters = new_counters }
+      { bf with counters = array_update bf.counters idx U8.(slot +^ 1uy) }
     end else
       { bf with counters = array_update bf.counters idx U8.(slot -^ 1uy) }
   else bf
@@ -85,7 +98,15 @@ val adjust_first_slot:
   bf:bloom_storage_u8 ->
   hash:u32 ->
   increment:bool{if not increment then not (first_slot_is_empty bf hash) else true} ->
-  Tot bloom_storage_u8
+  Tot (new_bf:bloom_storage_u8{
+    let idx = first_slot_index hash in
+    modified_only_one_slot bf new_bf idx /\
+    begin if increment then
+      not (slot_is_empty new_bf idx)
+    else
+      true
+    end
+  })
 let adjust_first_slot bf hash increment =
   adjust_slot bf (first_slot_index hash) increment
 
@@ -93,63 +114,172 @@ val adjust_second_slot:
   bf:bloom_storage_u8 ->
   hash:u32 ->
   increment:bool{if not increment then not (second_slot_is_empty bf hash) else true} ->
-  Tot bloom_storage_u8
+  Tot (new_bf:bloom_storage_u8{
+    let idx = second_slot_index hash in
+    modified_only_one_slot bf new_bf idx /\
+    begin if increment then
+      not (slot_is_empty new_bf idx)
+    else
+      true
+    end
+  })
 let adjust_second_slot bf hash increment =
   adjust_slot bf (second_slot_index hash) increment
 
-val insert_hash: bf:bloom_storage_u8 -> u32 -> Tot bloom_storage_u8
+let modified_hash_slots
+  (old_bf:bloom_storage_u8)
+  (new_bf:bloom_storage_u8)
+  (hash:u32) =
+  let idx1 = first_slot_index hash in
+  let idx2 = second_slot_index hash in
+  forall (idx':valid_index{idx' <> idx1 /\ idx' <> idx2}).
+  array_index new_bf.counters idx' = array_index old_bf.counters idx'
+
+val insert_hash:
+  bf:bloom_storage_u8 ->
+  hash: u32 ->
+  Tot (new_bf:bloom_storage_u8{
+    modified_hash_slots bf new_bf hash /\
+    might_contain_hash new_bf hash
+  })
 let insert_hash bf hash =
   let bf = adjust_first_slot bf hash true in
   adjust_second_slot bf hash true
 
-val remove_hash: bf:bloom_storage_u8 -> u32 -> Tot bloom_storage_u8
+val remove_hash:
+  bf:bloom_storage_u8 ->
+  hash:u32 ->
+  Tot (new_bf:bloom_storage_u8{modified_hash_slots bf new_bf hash})
 let remove_hash bf hash =
   (* BEGIN ADDED CODE *)
   (* They never check before substracting in the slots ! Negative overflow might occur *)
-  if (first_slot_is_empty bf hash) then bf else begin
+  if (first_slot_is_empty bf hash)  then bf else begin
   (* END ADDED CODE*)
     let bf = adjust_first_slot bf hash false in
     (* BEGIN ADDED CODE *)
-    if (second_slot_is_empty bf hash) then adjust_first_slot bf hash true else
-    (* END ADDED CODE *)
-    adjust_second_slot bf hash false
+    if (second_slot_is_empty bf hash) then begin
+      adjust_first_slot bf hash true
+    end else
+      (* END ADDED CODE *)
+      adjust_second_slot bf hash false
   end
 
-val might_contain_hash: bf:bloom_storage_u8 -> u32 -> bool
-let might_contain_hash bf hash =
-  not (first_slot_is_empty bf hash) &&
-  not (second_slot_is_empty bf hash)
+let lemma_remove_hash_prelim
+  (bf: bloom_storage_u8)
+  (removed_hash: u32)
+  (idx: valid_index)
+  : Lemma (requires (
+    let new_bf = remove_hash bf removed_hash in
+    slot_is_empty new_bf idx /\
+    not (slot_is_empty bf idx)
+  ))
+  (ensures (False)) =
+    (* Here we prove by contradiction that
+       slot_is_empty bf idx ! *)
+    let new_bf = remove_hash bf removed_hash in
+    if (first_slot_is_empty bf removed_hash) then
+      ()
+    else begin
+      let bf' = adjust_first_slot bf removed_hash false in
+      if (second_slot_is_empty bf' removed_hash) then
+	()
+      else begin
+        let new_bf' = adjust_second_slot bf' removed_hash false in
+        assert (new_bf' = new_bf);
+	(* Only this case is tricky *)
+	if idx <> (first_slot_index removed_hash) &&
+	  idx <> (second_slot_index removed_hash)
+	then
+	  ()
+	else
+	  admit()//We lack a lemma that says that decrementing an empty bucket will cause it to
+	  // remain empty
+      end
+    end
 
+let lemma_remove_hash1
+  (bf: bloom_storage_u8)
+  (removed_hash: u32)
+  (hash: u32)
+  : Lemma (requires (
+    first_slot_is_empty (remove_hash bf removed_hash) hash
+  ))
+  (ensures (first_slot_is_empty bf hash)) =
+    if not (first_slot_is_empty bf hash) then
+    lemma_remove_hash_prelim bf removed_hash (first_slot_index hash)
 
-let is_valid_bloom_filter (bf: bloom_storage_u8) : Tot bool =
-  let elements = bf.ghost_state.elements in
-  all_elements elements (fun (e, _) ->
-    might_contain_hash bf (hash e)
-  )
-
-type valid_bloom_storage_u8 = bf:bloom_storage_u8{is_valid_bloom_filter bf}
+let lemma_remove_hash2
+  (bf: bloom_storage_u8)
+  (removed_hash: u32)
+  (hash:u32)
+  : Lemma (requires (
+    second_slot_is_empty (remove_hash bf removed_hash) hash
+  ))
+  (ensures (
+    second_slot_is_empty bf hash
+  )) =
+  if not (second_slot_is_empty bf hash) then
+    lemma_remove_hash_prelim bf removed_hash (second_slot_index hash)
 
 val is_zeroed: bf:bloom_storage_u8 -> Tot bool
 let is_zeroed bf =
   vec_all bf.counters (fun x -> x = 0uy)
 
-val insert_element: bf:valid_bloom_storage_u8 -> element -> Tot valid_bloom_storage_u8
+let add_only_bloom_filter (bf: bloom_storage_u8) : Tot bool =
+  let elements = bf.ghost_state.elements in
+  all_elements elements (fun e ->
+    might_contain_hash bf (hash e)
+  )
+
+let element_invalidation (bf: bloom_storage_u8) =
+  (forall (e:element). (
+    (not (might_contain_hash bf (hash e))) ==>
+      (not (contains bf.ghost_state.elements e))
+  ))
+
+let lemma_add_only_bloom_filter
+  (bf: bloom_storage_u8)
+  : Lemma (ensures (
+    add_only_bloom_filter bf <==>
+    (forall (e:element{contains bf.ghost_state.elements e}).
+      might_contain_hash bf (hash e))
+  )) =
+    all_elements_lemma
+      #element
+      bf.ghost_state.elements
+      (fun e -> might_contain_hash bf (hash e))
+
+type valid_bloom_storage_u8 = bf:bloom_storage_u8{element_invalidation bf}
+
+type add_only_bloom_storage_u8 = bf:valid_bloom_storage_u8{add_only_bloom_filter bf}
+
+val insert_element: bf:add_only_bloom_storage_u8 -> element -> Tot add_only_bloom_storage_u8
 let insert_element bf e =
   let hash_val = hash e in
-  let bf = { bf with ghost_state = spec_insert_element bf.ghost_state e } in
+  (* *) let new_bf = { bf with ghost_state = spec_insert_element bf.ghost_state e } in
   let new_bf = insert_hash bf hash_val in
-  (* *)
-  let elements = bf.ghost_state.elements in
-  all_elements elements (fun (e', _) ->
-    let cond = might_contain_hash bf (hash e') in
-    if e <> e' then assert(cond) else ();
-    cond
-  );
-  admit();
+  (* *) lemma_add_only_bloom_filter bf;
+  (* *) lemma_add_only_bloom_filter new_bf;
   new_bf
 
 val remove_element: bf:valid_bloom_storage_u8 -> element -> Tot valid_bloom_storage_u8
 let remove_element bf e =
-  let hash = hash e in
-  let bf = { bf with ghost_state = spec_remove_element bf.ghost_state e } in
-  remove_hash bf hash
+  let hash_e = hash e in
+  let new_bf = { bf with ghost_state = spec_remove_element bf.ghost_state e } in
+  let new_bf = remove_hash bf hash_e in
+  (* *) let inner_lemma
+  (* *)   (e':element{not (might_contain_hash new_bf (hash e'))})
+  (* *)   : Lemma (ensures (not (contains new_bf.ghost_state.elements e')))
+  (* *)   =
+  (* *)   let hash_e' = hash e' in
+  (* *)   Classical.or_elim
+  (* *)     #(first_slot_is_empty new_bf hash_e')
+  (* *)     #(second_slot_is_empty new_bf hash_e')
+  (* *)     #(fun _ -> first_slot_is_empty bf hash_e' \/
+  (* *)       second_slot_is_empty bf hash_e')
+  (* *)     (fun _ -> lemma_remove_hash1 bf hash_e hash_e')
+  (* *)     (fun _ -> lemma_remove_hash2 bf hash_e hash_e');
+  (* *)   ()
+  (* *) in
+  (* *) Classical.forall_intro inner_lemma;
+  new_bf
