bloom-filter/Spec.BloomFilter.fst
@@ -15,7 +15,7 @@ assume type element: eqtype
 
 assume val hash: element -> u32
 
-type count = n:nat{n > 0}
+type count = n:int
 
 let contains (#a:eqtype) (l:list (a & count)) (e:a) : Tot bool =
   existsb (fun (e', _) -> e = e') l
@@ -47,7 +47,7 @@ let rec incr_count #a l e =
 val element_count: #a:eqtype ->
   l:count_list a ->
   e: a ->
-  Tot nat (decreases l)
+  Tot count (decreases l)
 let rec element_count #a l e = match l with
   | [] -> 0
   | (e', count)::tl ->
@@ -58,37 +58,94 @@ val decr_count:
   l:count_list a ->
   e : a{contains l e} ->
   Tot (l':count_list a{
-    if element_count l e > 1 then
       same_elements l l'
-    else begin
-      not (contains l' e) /\
-      (forall (e':a{e' <> e}). contains l e' <==> contains l' e')
-    end
   }) (decreases l)
 let rec decr_count #a l e =
   match l with
   | [] -> l
   | (e', old_count)::tl ->
-    if e = e' && old_count = 1 then
-      tl
-    else if e = e' && old_count > 1 then
+    if e = e' then
       (e', old_count - 1)::tl
     else
       (e', old_count)::(decr_count tl e)
 
-noeq type spec_bloom_storage_u8 = {
+type spec_bloom_storage_u8 = {
    elements: (l:(count_list element){no_duplicates l})
 }
 
 let rec all_elements
   (#a:eqtype)
   (l:count_list a)
-  (f:((a & count) -> bool))
-  : Tot bool (decreases l) =
+  (f:a -> bool)
+  : Tot (b:bool) (decreases l) =
   match l with
   | [] -> true
-  | hd::tl -> if f hd then all_elements tl f else false
+  | (hd,_)::tl -> if f hd then all_elements tl f else false
 
+let rec all_elements_lemma1
+  (#a:eqtype)
+  (l: count_list a)
+  (f:a -> bool)
+  : Lemma (ensures (
+    all_elements #a l f ==>
+      (forall (e:a{contains l e}). f e)
+    )) (decreases l)
+  =
+  if not (all_elements #a l f) then () else
+  match l with
+  | [] -> ()
+  | (e_hd,_)::tl ->
+    assert (not (contains tl e_hd));
+    if not (f e_hd) then assert(false) else begin
+      let inner_lemma
+	(e:a{contains l e})
+	: Lemma (ensures (f e)) =
+	assert (e = e_hd \/ contains tl e);
+	Classical.or_elim
+	  #(e = e_hd)
+	  #(contains tl e)
+	  #(fun _ -> f e)
+	  (fun _ -> assert (e = e_hd))
+	  (fun _ -> assert (contains tl e);
+	    all_elements_lemma1 #a tl f
+	  )
+      in
+      Classical.forall_intro inner_lemma
+    end
+
+let rec all_elements_lemma2
+  (#a:eqtype)
+  (l: count_list a)
+  (f:a -> bool)
+  : Lemma (ensures (
+    (forall (e:a{contains l e}). f e) ==>
+      all_elements #a l f
+    )) (decreases l)
+  =
+  let rec inner_lemma
+    (_ : (forall (e:a{contains l e}). f e))
+    : Lemma (ensures (all_elements #a l f))
+    = match l with
+    | [] -> ()
+    | (hd, _)::tl -> all_elements_lemma2 #a tl f
+  in
+  Classical.impl_intro
+    #((forall (e:a{contains l e}). f e))
+    #(all_elements #a l f)
+    inner_lemma
+
+
+let rec all_elements_lemma
+  (#a:eqtype)
+  (l: count_list a)
+  (f:a -> bool)
+  : Lemma (ensures (
+    all_elements #a l f <==>
+      (forall (e:a{contains l e}). f e)
+    )) (decreases l)
+  =
+  all_elements_lemma1 #a l f;
+  all_elements_lemma2 #a l f
 
 val spec_insert_element:
   bf:spec_bloom_storage_u8 ->
@@ -100,6 +157,18 @@ let spec_insert_element bf e =
   else
     { bf with elements = (e,1)::bf.elements }
 
+let lemma_spec_insert_element
+  (bf:spec_bloom_storage_u8)
+  (e:element)
+  : Lemma (ensures (
+    let new_bf = spec_insert_element bf e in
+    (forall(e':element{e' <> e}).
+      (contains bf.elements e' <==> contains new_bf.elements e'))
+    /\ contains new_bf.elements e
+  )) =
+  ()
+
+
 val spec_remove_element:
   bf:spec_bloom_storage_u8 ->
   e:element ->
@@ -109,3 +178,12 @@ let spec_remove_element bf e =
     { bf with elements = decr_count bf.elements e }
   else
     bf
+
+let lemma_spec_remove_element
+  (bf:spec_bloom_storage_u8)
+  (e:element)
+  : Lemma (ensures (
+    let new_bf = spec_remove_element bf e in
+    same_elements bf.elements new_bf.elements
+  )) =
+  ()
